@prefix : <https://github.com/AKSW/leds-asp-f-ontologies#> .
@prefix owl: <http://www.w3.org/2002/07/owl#> .
@prefix rdf: <http://www.w3.org/1999/02/22-rdf-syntax-ns#> .
@prefix xml: <http://www.w3.org/XML/1998/namespace> .
@prefix xsd: <http://www.w3.org/2001/XMLSchema#> .
@prefix rdfs: <http://www.w3.org/2000/01/rdf-schema#> .

<https://github.com/AKSW/leds-asp-f-ontologies> a owl:Ontology .
# 
# 
# #################################################################
# #
# #    Object Properties
# #
# #################################################################
# 
# 
# https://github.com/AKSW/leds-asp-f-ontologies#accessible_from_floor

:accessible_from_floor a owl:ObjectProperty ;
	rdfs:domain :Building_Part ;
	rdfs:range :Floor .
# 
# https://github.com/AKSW/leds-asp-f-ontologies#accessible_through_entrance

:accessible_through_entrance a owl:ObjectProperty ;
	rdfs:domain :Building ;
	rdfs:range :Entrance .
# 
# https://github.com/AKSW/leds-asp-f-ontologies#contains_obstacle

:contains_obstacle a owl:ObjectProperty ;
	rdfs:subPropertyOf owl:topObjectProperty ;
	rdfs:domain :Building_Part ;
	rdfs:range :Obstacle .
# 
# https://github.com/AKSW/leds-asp-f-ontologies#has_building_part

:has_building_part a owl:ObjectProperty ;
	rdfs:domain :Building ;
	rdfs:range :Building_Part .
# 
# https://github.com/AKSW/leds-asp-f-ontologies#has_entrance_direction

:has_entrance_direction a owl:ObjectProperty ;
	rdfs:domain :Entrance ;
	rdfs:range :Entrance_Direction .
# 
# https://github.com/AKSW/leds-asp-f-ontologies#has_floor

:has_floor a owl:ObjectProperty ;
	rdfs:domain :Building ;
	rdfs:range :Floor .
# 
# https://github.com/AKSW/leds-asp-f-ontologies#has_location

:has_location a owl:ObjectProperty ;
	rdfs:domain :Building ;
	rdfs:range :Location_Information .
# 
# https://github.com/AKSW/leds-asp-f-ontologies#is_Entrance

:is_Entrance a owl:ObjectProperty ;
	rdfs:domain :Building_Part ;
	rdfs:range :Entrance .
# 
# https://github.com/AKSW/leds-asp-f-ontologies#is_connected_to

:is_connected_to a owl:ObjectProperty ;
	rdfs:domain :Building_Part ;
	rdfs:range :Building_Part .
# 
# https://github.com/AKSW/leds-asp-f-ontologies#is_point_of_interest

:is_point_of_interest a owl:ObjectProperty ;
	rdfs:domain :Building_Part ;
	rdfs:range :Point_of_Interest .
# 
# 
# 
# #################################################################
# #
# #    Classes
# #
# #################################################################
# 
# 
# https://github.com/AKSW/leds-asp-f-ontologies#Building

:Building a owl:Class ;
	rdfs:subClassOf :Space ;
	rdfs:comment "A Building is a spacial instance that is artificial and made for human inhabitants. It's usually has a roof and speparated from the environment by walls and doors."@en ;
	rdfs:label "Gebaeude"@de .
# 
# https://github.com/AKSW/leds-asp-f-ontologies#Building_Part

:Building_Part a owl:Class ;
	rdfs:subClassOf :Space ;
	rdfs:comment "A Building Part is a spatial sub unit of a building."@en ;
	rdfs:label "Gebaeudeteil"@de .
# 
# https://github.com/AKSW/leds-asp-f-ontologies#Door

:Door a owl:Class ;
	rdfs:subClassOf :Building_Part ;
	rdfs:comment "A Door is a moveable object between spatial instances. It's generally used for blocking access to unauthorized persons. It may just isolate thermally, acustically or/and optically. It's movability is usually limited to rotation on hinges and wall and frame placement."@en ;
	rdfs:label "Tuer"@de .
# 
# https://github.com/AKSW/leds-asp-f-ontologies#Elevator

:Elevator a owl:Class ;
	rdfs:subClassOf :Building_Part ;
	rdfs:comment "An Elevator is a shaft with a movable cabin to transport persons horizontally."@en ;
	rdfs:label "Aufzug"@de .
# 
# https://github.com/AKSW/leds-asp-f-ontologies#Entrance

:Entrance a owl:Class ;
	rdfs:comment "Entrance is a transition between a building interrior space and building outside space."@en ;
	rdfs:label "Eingang"@de .
# 
# https://github.com/AKSW/leds-asp-f-ontologies#Entrance_Direction

:Entrance_Direction a owl:Class ;
	rdfs:comment "Entrance Direction is an additional Information for an Entrance. It's the direction in which the entrance is supposed to be used."@en ;
	rdfs:label "Zugangsrichtung"@de .
# 
# https://github.com/AKSW/leds-asp-f-ontologies#Escalator

:Escalator a owl:Class ;
	rdfs:subClassOf :Building_Part ;
	rdfs:comment "An Escalator is a transportation system for horizontal transit. It's usually used for transition between floors."@en ;
	rdfs:label "Rolltreppe"@de .
# 
# https://github.com/AKSW/leds-asp-f-ontologies#Floor

:Floor a owl:Class ;
	rdfs:subClassOf :Space ;
	rdfs:comment "Floor is a story of a building. It's used to decribe a spatial layer which has mostly no vertical transitions."@en ;
	rdfs:label "Etage"@de .
# 
# https://github.com/AKSW/leds-asp-f-ontologies#Location_Information

:Location_Information a owl:Class ;
	rdfs:comment "Location is a information group for locating descriptions. E.g. coordinates, hight, address and so on."@en ;
	rdfs:label "Standortinformationen"@de .
# 
# https://github.com/AKSW/leds-asp-f-ontologies#Obstacle

:Obstacle a owl:Class ;
	rdfs:comment "Obstacle is a thing, void or situation that keeps a person or vehicle from unrestraint movement."@en ;
	rdfs:label "Hindernis"@de .
# 
# https://github.com/AKSW/leds-asp-f-ontologies#Point_of_Interest

:Point_of_Interest a owl:Class ;
	rdfs:comment "Point of Interest is an abstract location which is may be useful or interesting for a service or person."@en ;
	rdfs:label "Interessensfokus"@de .
# 
# https://github.com/AKSW/leds-asp-f-ontologies#Ramp

:Ramp a owl:Class ;
	rdfs:subClassOf :Building_Part ;
	rdfs:comment "A Ramp, also called wheelchair ramp, is a plane that is angled to overcome verticale hight differences."@en ;
	rdfs:label "Rampe"@de .
# 
# https://github.com/AKSW/leds-asp-f-ontologies#Room

:Room a owl:Class ;
	rdfs:subClassOf :Building_Part ;
	rdfs:comment "A Room is a spatial instance that is used for storing, living, working or waiting within. It's also a used for transitioning into other spaces."@en ;
	rdfs:label "hausinterner Raum"@de .
# 
# https://github.com/AKSW/leds-asp-f-ontologies#Space

:Space a owl:Class ;
	rdfs:comment "Sapce is everything that describes a spatial instance."@en ;
	rdfs:label "Raum"@de .
# 
# 
# 
# #################################################################
# #
# #    Individuals
# #
# #################################################################
# 
# 
# https://github.com/AKSW/leds-asp-f-ontologies#bidirectional

:bidirectional a owl:NamedIndividual .
# 
# https://github.com/AKSW/leds-asp-f-ontologies#in

:in a owl:NamedIndividual .
# 
# https://github.com/AKSW/leds-asp-f-ontologies#out

:out a owl:NamedIndividual .
# 
# https://github.com/AKSW/leds-asp-f-ontologies#out_(emergency_exit)

<https://github.com/AKSW/leds-asp-f-ontologies#out_(emergency_exit)> a owl:NamedIndividual .
# 
# Generated by the OWL API (version 4.2.5.20160517-0735) https://github.com/owlcs/owlapi
